---
title: Measure Spaces
author: Colton Grainger (MATH 6130 Analysis)
date: 2018-09-16
bibliography: /home/colton/Downloads/coltongrainger.bib
macros: true
---

\setcounter{section}{1}

## Assignment due 2018-09-26

### Finite coverings of a measure space

Let $\{E_i\}_{i=1}^n$ be a finite sequence of measurable subsets of the measure space $(X, \sM, \mu)$, where $\mu(X) = 1$. If each point of $X$ belongs to at least three of these sets, then at least one of the $E_i$ has measure greater than or equal to $\frac3n$.

*Proof.* Partition $X$ by taking the minimal elements in the finite algebra $\sA$ generated by the $E_i$ in $X$ (partially ordered by set inclusion). Let the finite collection of such minimal elements be $\sC$. For each $C_j \in \sC$, we observe that $C_j \in \sM$. Furthermore, $\sC$ partitions $X$ because (i) the $E_i$ cover $X$ and (ii) if two blocks $C_j$ and  $C_k$ in $\sC$ did intersect, these blocks would not minimal elements in $\sA$, a contradiction. We conclude that every point in $X$ belongs to exactly one of finitely many $C_j \in \sC$.

For notation's sake, let $C_j^i = E_i \cap C_j$ for all $i=1,\ldots,n$ and all $j$. Now every point in $X$ is, by hypothesis, contained in at least three of the $E_i$, whence also contained in at least three of the $C_j^i$. There are thus at least three values of $j$ for which $\{C_j^i\}_{i=1}^n$ is a partition of $X$. With $\mu(X) = 1$, finite additivity implies

$$\sum_{i=1}^n\sum_{\forall j} \mu(C_j^i) \geq 3\mu(X) = 3.$$

But by construction $E_i = \sqcup_{\forall j} C_j^i$. Hence, by finite additivity, 
$$\sum_{i=1}^n \mu(E_i) = \sum_{i=1}^n\sum_{\forall j} \mu(C_j^i).$$

We conclude that $\sum_{i=1}^n \mu(E_i) \geq 3$, so there's a $E_i$ with $\mu(E_i) \ge \frac{3}{n}.$ \qedsymbol

### Equivalence relations on a finite space [@Fo99, number 1.12]

Let $(X, \sM, \mu)$ be a finite measure space.

(a) If $E, F \in \sM$ and $\mu(E\triangle F)=0$, then $\mu(E) = \mu(F)$.
(b) Say that $E \sim F$ iff $\mu(E \triangle F) = 0$: then $\sim$ is an equivalence relation on $\sM$.
(c) If $E, F \in \sM$, define $\rho(E,F) = \mu(E \triangle F)$. Then $\rho(E,G)\le \rho(E,F) + \rho(F,G)$ for all $E,F,G \in \sM$, and hence $\rho$ defines a metric on the quotient space $\sM/\sim$.

*Proof.* Let $E, F$ be measurable sets, and suppose that $\mu(E\triangle F) = 0$. Since $$E \triangle F = (E \setminus F) \sqcup (F \setminus E)$$ from additivity we have $0 = \mu(E\triangle F) = \mu(E \setminus F) +  \mu(F \setminus E)$. Now $\mu$ maps into $[0,\infty]$, so both $\mu(E \setminus F) = \mu(F \setminus E) = 0$. Break into disjoint sets $E = (E \setminus F) \sqcup (E \cap F)$ and $F = (F \setminus E) \sqcup (F \cap E)$, so that, again by additivity, we prove (a)
\begin{align*}
\mu(E) &= \mu(E \setminus F) + \mu(E \cap F)\\
    &= \mu(E \cap F) + \mu(F \setminus F)\\
    &= \mu(F).
\end{align*}

For the relation defined on $\sM$ by $E \sim F$ iff $\mu(E \triangle F) = 0$,

- $E \sim E$ as $E \triangle E = \emptyset$ is a null set under $\mu$,
- $E \sim F$ implies $F \sim E$ as $E \triangle F = F \triangle E$,
- $E \sim F$ and $F \sim G$ implies $E \sim G$ as 
    $$E \triangle G 
    = (E \triangle F)\triangle(F \triangle G) 
    = [(E \triangle F) \setminus (F \triangle G)] \sqcup [ (F \triangle G) \setminus (E \triangle F) ]$$ 
  and when $\mu(E \triangle F) = \mu(F \triangle G) = 0$, we have (by monotonicity) $$\mu(E \triangle G) = \mu[(E \triangle F) \setminus (F \triangle G)] + \mu[ (F \triangle G) \setminus (E \triangle F)] \le \mu(E \triangle F) + \mu(F \triangle G) = 0.$$

Let $\bar{\sM}$ be the set of equivalence classes in $\sM$ by the relation $\sim$. To show the function $\rho \colon \bar{\sM} \times \bar{\sM} \to [0,\infty]$ defined by $\rho(\bar{E}, \bar{F}) = \mu(E \triangle F)$ is a metric, consider the equivalence classes of any three measurable sets $E$, $F$, and $G$. Because $\rho$ is defined on $\bar{\sM}$, we know $\rho(\bar{E}, \bar{F}) = 0$ iff $\mu(E \triangle F) = 0$ iff $\bar{E} = \bar{F}$. Because the binary operator $\triangle$ is symmetric, $\rho$ is symmetric. The triangle inequality on $\rho$ follows from $\mu(E \triangle G) \leq \mu(E \triangle F) + \mu(F \triangle G)$. Therefore $\rho$ is a metric on $\bar{\sM}$.

### Large sets in semifinite measures [@Fo99, number 1.14] 

If $\mu$ is a semifinite measure and $\mu(E) = \infty$, then for any $C > 0$ there exists $F \subset E$ with $C < \mu(F) < \infty$.

*Proof*. Because $\mu$ is semifinite, for any $E \in \sM$ such that $\mu(E) = \infty$ the set $$\sF = \{ F \subset E : F \text{ is measurable and } 0 < \mu(F) < \mu(E)\}$$ is non-empty. So choose an arbitrary $E \in \sM$. Now consider $k = \sup_{F \in \sF} \mu(F)$. If $k = \infty$ the claim follows, because we would have, for all $C > 0$, some set $B \in \sF$ such that $\mu(B) > 0$. We therefore will suppose $k < \infty$ and proceed to find a sequence $\{F_i\}_1^\infty \subset \sF$ such that $\mu(\cup_1^\infty F_i) = \infty$.

For contradiction, suppose $k < \infty$ and there's no sequence $\{F_i\}$ in $\sF$ with $\mu(\cup F_i) = \infty$. Yet clearly there's a sequence $\{F_i\} \subset \sF$ such that $\mu(F_i) \to k$. For this sequence, by additivity, $$\mu(\cup F_i) + \mu(E \setminus \cup F_i) = \mu(E) = \infty.$$ We've assumed $\mu(\cup F_i) < \infty$, so for the previous equality to hold we must have $\mu(E \setminus \cup F_i) = \infty$. Because $\mu$ is semifinite, there's a set $G \in \sM$ such that $G \subset (E \setminus \cup F_i)$ and $0 < \mu(G) < \infty$. Observe that $G \sqcup (\cup F_i) \in \sF$. Hence the contradiction $$> k \ge \mu(G \sqcup (\cup F_i)) = \mu(G) + \mu(\cup F_i) > \mu(\cup F_i) \ge k$$ where we have $\mu(\cup F_i) \ge k$ as a consequence of monotonicity and continuity from below when $\mu(F_i) \to k$.

We have argued that there's a sequence $\{F_i\} \subset \sF$ such that $\mu(\cup F_i) = \infty$. As a direct result, we conclude that for all $C > 0$ there's an $n \in \NN$ such that $\mu(\cup_1^n F_i) > C$. \qedsymbol

### Semifinite parts [@Fo99, number 1.15]

\newcommand{\fmss}[1]{\mathrm{fmss}(#1)}

If $\mu$ is a measure on $(X, \sM)$, define $\mu_0(E)$ for each $E \in \sM$ by $$\mu_0(E) = \sup\{\mu(F) : F \subset E \text{ and } \mu(F) \le \infty\}.$$

(a) $\mu_0$ is a semifinite measure on $\sM$.^[It's called the **semifinite part** of $\mu$.]
(b) If $\mu$ is semifinite, then $\mu_0 = \mu$.

*Proof.* To introduce notation, let $\fmss{E}$ denote $\{\mu(F) : F \subset E \text{ and } \mu(F) \le \infty\}$, the set of measures of the "finite measure subsets" of E. Then define $\mu_0$ on $\sM$ by $\mu_0(E) = \sup\fmss{E}$. I claim $\mu_0$ inherits two properties from $\mu$, namely that

- $\mu_0$ assigns no mass to the empty set, and 
- $\mu_0$ has countable additivity.

We'll now argue $\mu_0$ is semifinite. Suppose that $\mu_0(E) =\infty$. We aim to show there's a subset $G \subset E$ such that $0 < \mu_0(G) < \mu_0(E)$. By definition of $\fmss{E}$ we know $\infty \notin \fmss{E}$. In order to have $\infty = \mu_0(E) = \sup\fmss{E}$ there must exist a sequence $\{F_j\}_1^\infty$ such that $F_j \subset E$, $\mu(F_j) < \infty$, and $\mu(F_j) \to \infty$.

Choose $G$ from the $F_j$ where $\mu(G) > 0$ (such a $G$ exists, for countable many of the $F_j$ have non-zero measure). Because $\mu(G) \in \fmss{G}$, we have $$\mu_0(G) = \sup\fmss{G} \ge \mu(G) > 0.$$ Can $\mu_0(G) = \infty$? No, by monotonicity, $\mu(G)$ is a finite upper bound for $\fmss{G}$, and therefore $$\mu_0(G) = \sup \fmss{G} \le \mu(G) = \mu(F_{j'}) < \infty.$$ Because we have $G \subset E$ and $0 < \mu_0(G) < \infty$, we conclude $\mu_0$ is a semifinite measure, proving (a).

Assume now that $\mu$ is semifinite. Take an arbitrary $E \in \sM$. We argue that $\mu_0 = \mu$ in three cases:

1. Suppose $\mu(E) < \infty$. Then $\mu(E) \in \fmss{E}$. Then $\mu_0(E) := \sup \fmss{E} \ge \mu(E)$. By monotonicity, if $F \subset E$ then $\mu(F) \le \mu(E)$. So $\mu(E)$ is an upper bound for $\fmss{E}$. Then $\mu_0(E):= \sup\fmss{E} \le \mu(E)$. 
2. In the case that $\mu_0(E) = \infty$, because $\mu(E)$ is an upper bound for $\fmss{E}$ we have $\infty = \mu_0(E) \le \mu(E)$.
3. Lastly, suppose $\mu(E) = \infty$. Since $\mu$ is a semifinite measure, by previous exercise (large sets in semifinite measures), there's an unbounded sequence of values in $\fmss{E}$. Thence $\mu_0(E) := \sup\fmss{E} = \infty$.

We conclude that $\mu = \mu_0$, proving (b). \qedsymbol

### Countable additivity for intersections in outer measures [@Fo99, number 1.17]

If $\mu^*$ is an outer measure and $\{A_j\}_1^\infty$ is a sequence of disjoint $\mu^*$-measurable sets, then $\mu^*(E \cap (\cup_1^\infty A_j)) = \sum_1^\infty \mu^*(E\cap A_j)$ for any $E \subset X$.

\newcommand{\msbl}{$\mu^*$-measurable}

*Proof.* Let $E \subset X$ and consider an arbitrary disjoint sequence $\{A_j\}_1^\infty$ of \msbl\ sets. We'll proceed by strong induction on the number of $A_j$ in the union $\cup_1^n A_j$.

For a base case, we have the tautology: $\mu^*(A_1 \cap E) = \sum_1^1 \mu^*(A_j \cap E).$ Now assume for natural numbers $k < n$ that $\mu^*(E \cap (\cup_1^k A_j)) = \sum_1^k \mu^*(E\cap A_j)$. By CarathÃ©odory's theorem, we have that $\mu^*$ restricted to \msbl\ sets is a measure. So noting $A_{n} \cap E$ is \msbl\ with each $A_j \cap E$ disjoint, we have additivity. Thus 
$$\mu^*\left(\cup_{j=1}^{n} A_j \cap E\right) = \mu^*\left(\left(\cup_{j=1}^{n-1} A_j \cap E\right) \sqcup \left(\cup_{j=1}^{n-1} A_j \cap E\right)\right) = \sum_{j=1}^{n-1} \mu^*(A_j \cap E) + \mu^*(A_{k+1} \cap E) = \sum_{j=1}^{n} \mu^*(A_j \cap E).$$

Assuming that $E \cap A_j$ is \msbl for any $j$, we are done. \qedsymbol

## References
